added find_goals method and rewrote focus method to just use match.

lib/Eisbach_Methods.thy
@@ -6,19 +6,7 @@ imports "~~/src/HOL/Eisbach/Eisbach_Tools"
         "subgoal_focus/Subgoal_Methods"
 begin
 
-ML \<open>fun DROP_CASES f xq = (Seq.map snd o f) xq\<close>
 
-(* Focus without matching. No focus elements are available directly. *)
-method_setup focus = \<open>
-  Scan.lift (Args.mode "concl") -- Method_Closure.parse_method >> (fn (b,m) => fn ctxt => fn facts => 
-  let
-    val m' = Method_Closure.method_evaluate m;
-    val focus = if b then Subgoal.FOCUS else Subgoal.FOCUS_PARAMS; 
-  in
-   focus (fn {context,...} => DROP_CASES (m' context facts)) ctxt 1
-   |> EMPTY_CASES
-   end)
-\<close>
 
 method_setup all =
  \<open>Method_Closure.parse_method >> (fn m => fn ctxt => fn facts =>
@@ -37,6 +25,38 @@ method_setup print_goal = \<open>Scan.succeed (fn ctxt => fn facts =>
   (fn st => (Output.writeln (Display.string_of_thm ctxt st); Seq.single ([],st))))\<close>
 
 
+
+
+(* lift methods into logical tests *)
+
+method_setup fails =
+ \<open>Method_Closure.parse_method >> (fn m => fn ctxt => fn facts =>
+   let
+     fun fail_tac st' = 
+       (case Seq.pull (Method_Closure.method_evaluate m ctxt facts st') of
+          SOME _ => Seq.empty
+        | NONE => Seq.single st')
+
+   in EMPTY_CASES fail_tac end)
+\<close>
+
+method_setup succeeds =
+ \<open>Method_Closure.parse_method >> (fn m => fn ctxt => fn facts =>
+   let
+     fun can_tac st' = 
+       (case Seq.pull (Method_Closure.method_evaluate m ctxt facts st') of
+          SOME (st'',_) => Seq.single st'
+        | NONE => Seq.empty)
+
+   in EMPTY_CASES can_tac end)
+\<close>
+
+(* focus without matching *)
+
+method focus_concl methods m =
+  ((fails \<open>erule thin_rl\<close>, match conclusion in _ \<Rightarrow> \<open>m\<close>)
+  | match premises in H:_ (multi) \<Rightarrow> \<open>m\<close>)
+
 context
 begin
 
@@ -50,14 +70,76 @@ private lemma protect_end: "protect_concl P \<Longrightarrow> P \<Longrightarrow
   by (simp add: protect_concl_def protect_false_def)
 
 method only_asm methods m = 
-  (match premises in H[thin]:_ (multi) \<Rightarrow> 
+  (match premises in H[thin]:_ (multi,cut) \<Rightarrow> 
     \<open>rule protect_start, 
      match premises in H'[thin]:"protect_concl _" \<Rightarrow> 
        \<open>insert H,m;rule protect_end[OF H']\<close>\<close>)
 
-method only_concl methods m = (match premises in _ (multi) \<Rightarrow> \<open>m\<close>)
+method only_concl methods m = (focus_concl \<open>m\<close>)
 
 end
+
+context begin
+
+private definition "goal_tag (x :: unit) \<equiv> TERM x"
+
+private lemma goal_tagI: "PROP goal_tag x"
+  unfolding goal_tag_def
+  by (rule termI)
+
+private method make_tag_goal for tag_id :: unit = (rule thin_rl[of "PROP goal_tag tag_id"])
+
+private method clear_tagged_goal for tag_id :: unit  = (rule goal_tagI[of tag_id])
+
+private definition "goals_end \<equiv> ()"
+private definition "method_succeed \<equiv> ()"
+private definition "method_failure \<equiv> ()"
+
+
+private method defer_tac = tactic \<open>defer_tac 1\<close>
+
+method find_goal methods m = 
+  (make_tag_goal goals_end, 
+   defer_tac,
+   (fails \<open>clear_tagged_goal method_succeed | clear_tagged_goal goals_end\<close>,
+     (((m)[1],make_tag_goal method_succeed) 
+     | defer_tac))+,
+   clear_tagged_goal method_succeed,
+   all \<open>(clear_tagged_goal goals_end)?\<close>)
+
+end
+
+(* examples *)
+
+notepad begin
+
+  fix A B
+  assume A: "A" and B: "B"
+
+  have "A" "A" "B"
+    apply (find_goal \<open>match conclusion in B \<Rightarrow> \<open>-\<close>\<close>)
+    apply (rule B)
+    by (rule A)+
+
+  have "A \<and> A" "A \<and> A" "B"
+    apply (find_goal \<open>fails \<open>simp\<close>\<close>) (* find the first goal which cannot be simplified *)
+    apply (rule B)
+    by (simp add: A)+
+
+  have  "B" "A" "A \<and> A"
+    apply (find_goal \<open>succeeds \<open>simp\<close>\<close>) (* find the first goal which can be simplified (without doing so) *)
+    apply (rule conjI)
+    by (rule A B)+
+
+
+  fix D C
+  assume DC:"D \<Longrightarrow> C"
+  have "D \<and> D \<Longrightarrow> C \<and> C"
+  apply (only_asm \<open>simp\<close>) (* stash conclusion before applying method *)
+  apply (only_concl \<open>simp add: DC\<close>) (* hide premises from method *)
+  by (rule DC)
+end
+    
 
 
 end
